# ajoeiwf
## ajoeiwf
## ajoeiwf

-------

| oaejfoijaewiofi | aweijfae | 
| --------------- | -------- | 
| aewfij          | aweijfae |
| aewfij          | aweijfae | 
| aewfij          | aweijfae | 
| aewfij          | aweijfae | 
| aewfij          | aweijfae | 


This is why you should *not* do __this__ alright...

$$ % Lines: 10
\displaylines{
    \sum_{n=-200}^{2} f(x) \\
    \frac{d}{dx} f(x) = x^2 + 2x^3 + 3 \\
    y = s + 1
}
$$
$$
x = y \cdot k
$$
$$ % Lines: 15
\begin{aligned}
y(x) &= \frac{x + 3}{x^2 + 3x + 2} \\
y^{'}(x) &= \frac{d}{dx} \left( \frac{x + 3}{x^2 + 3x + 2} \right) \\
         &= \frac{\left(x^2 + 3x + 2\right)\frac{d}{dx} \left( x + 3 \right) - \frac{d}{dx} \left(x^2 + 3x + 2\right)\left( x + 3 \right) } {\left( x^2 + 3x + 2 \right) ^ 2} \\
         &= \frac{\left(x^2 + 3x + 2\right) - \left(2x + 3 \right)\left( x + 3 \right) } {\left( x^2 + 3x + 2 \right) ^ 2} \\
         &= \frac{\left(x^2 + 3x + 2\right) - \left(2x^2 + 9x + 9 \right) } {\left( x^2 + 3x + 2 \right) ^ 2} \\
         &= \frac{-x^2 - 6x - 7} {\left( x^2 + 3x + 2 \right) ^ {10}} \\
\end{aligned}
$$


$$ % Lines: 1
\displaylines{
\neg\exists x \forall y (x > y) f(x)
}
$$


- aoijfe

> [!CAUTION]
> ajoeiwf

```rust
pub fn main() {

}
```
